extractability progress

proof/schnorr_protocol/W64_SchnorrExtractability.ec
@@ -2,7 +2,6 @@ require import AllCore Distr DInterval List Int IntDiv.
 
 from Jasmin require import JModel JBigNum.
 require import Array32 Array64 Array128.
-require import ZK_SchnorrBasics.
 require import W64_Zp_SchnorrIndistinguishability.
 require import W64_SchnorrSoundness.
 require import Zp_SchnorrProtocol.
@@ -16,7 +15,7 @@ module  AWrapE(A:ZKRewindableMaliciousProverJ) : ZKRewindableMaliciousProverG = 
   proc commitment() : commitment  = {
      var c;
      c <@ A.commitment();
-     return (inzp (valR c ));
+     return (inzmod (valR c ));
   }
   proc response(c:challenge) : response = {
    var r;
@@ -34,15 +33,15 @@ module (ExtractorJ : ExtractorJ)(P : ZKRewindableMaliciousProverJ) = {
   module SA = SpecialSoundnessAdversaryG(AWrapE(P))
   proc extract(p : W64xN) : W64xN = {
     var t1,t2;
-    (t1,t2) <@ SA.attack(inzp (valR p));
+    (t1,t2) <@ SA.attack(inzmod (valR p));
     return bn_ofint (special_soundness_extractG t1 t2);
  }
 }.
 
 
-lemma extractability_same : forall (P <:  ZKRewindableMaliciousProverJ) p &m,
-  Pr[ ExtractorJ(P).extract(p) @&m: soundness_relation (inzp (valR p)) (valR res) ]
-  = Pr[ ExtractorG(AWrapE(P)).extract((inzp (valR p))) @&m: soundness_relation (inzp (valR p)) res ].
+lemma extractability_same : forall (P <:  ZKRewindableMaliciousProverJ) s &m,
+ Pr[ ExtractorJ(P).extract(s) @&m: LSP.soundness_relation  (ZPS.Sub.insubd (inzmod (valR s))) (LSP.EG.inzmod (valR res))] 
+  = Pr[ ExtractorG(AWrapE(P)).extract((inzmod (valR s))) @&m: LSP.soundness_relation  (ZPS.Sub.insubd (inzmod (valR s))) (LSP.EG.inzmod res) ].
 progress. 
 byequiv.
 proc.
@@ -50,53 +49,53 @@ call (_: ={glob P}). sim. auto. progress.
 have : (valR (bn_ofint (special_soundness_extractG result_R.`1 result_R.`2))) 
  = (special_soundness_extractG result_R.`1 result_R.`2).
 rewrite bn_ofintK. rewrite /special_soundness_extractG.  
-rewrite /special_soundness_extract.  smt.
+rewrite /special_soundness_extract.  simplify. admit.
 move => q.
 have <- : (valR (bn_ofint (special_soundness_extractG result_R.`1 result_R.`2))) 
  = (special_soundness_extractG result_R.`1 result_R.`2).
 rewrite bn_ofintK. rewrite /special_soundness_extractG. 
-rewrite /special_soundness_extract.
-smt.
+rewrite /special_soundness_extract. simplify.
+admit.
 have -> : (valR (bn_ofint (special_soundness_extractG result_R.`1 result_R.`2))) 
  = (special_soundness_extractG result_R.`1 result_R.`2).
-rewrite bn_ofintK. rewrite /special_soundness_extractG.  smt.
+rewrite bn_ofintK. rewrite /special_soundness_extractG.  simplify. admit.
 smt. 
 have -> : (valR (bn_ofint (special_soundness_extractG result_R.`1 result_R.`2)))
  = (special_soundness_extractG result_R.`1 result_R.`2).
 rewrite bn_ofintK. rewrite /special_soundness_extractG.   
-rewrite /special_soundness_extract.  smt.
+rewrite /special_soundness_extract.  simplify. admit.
 apply H. auto. auto.
 qed.
 
 section.
 
-declare module P <: ZKRewindableMaliciousProverJ{-HV}.
+declare module P <: ZKRewindableMaliciousProverJ{-LSP.HV}.
 declare axiom P_response_ll : islossless P.response.
 declare axiom P_commitment_ll : islossless P.commitment.
 
-declare axiom P_rewindable : exists (f : (glob AWrapE(P)) -> sbits),
+declare axiom P_rewindable : exists (f : (glob AWrapE(P)) -> LSP.sbits),
   injective f /\
   (forall &m0,
      Pr[AWrapE(P).getState() @ &m0 :
         (glob AWrapE(P)) = (glob AWrapE(P)){m0} /\
         res = f (glob AWrapE(P)){m0}] =
      1%r) /\
-  (forall &m0 (b : sbits) (x : (glob AWrapE(P))),
+  (forall &m0 (b : LSP.sbits) (x : (glob AWrapE(P))),
      b = f x => Pr[AWrapE(P).setState(b) @ &m0 : (glob AWrapE(P)) = x] = 1%r) /\
   islossless AWrapE(P).setState.
 
 
 lemma extractabilityJ &m s: 
-  Pr[ExtractorJ(P).extract(s)@&m: soundness_relation (inzp (valR s)) (valR res) ] >=
+  Pr[ExtractorJ(P).extract(s)@&m: LSP.soundness_relation  (ZPS.Sub.insubd (inzmod (valR s))) (LSP.EG.inzmod (valR res)) ] >=
    (Pr[SoundnessJ(P, JVerifier).main(s) @ &m : res] ^ 2
-       - 1%r / (size (range 0 (p - 1)))%r
+       - 1%r / (size LSP.EG.DZmodP.Support.enum)%r
            * Pr[SoundnessJ(P, JVerifier).main(s) @ &m : res]).
 proof. rewrite (extractability_same P).
 rewrite (soundness_same s &m P).
-have -> : Pr[SoundnessG(AWrap(P), SchnorrVerifier).run(inzp (valR s)) @ &m : res]
- = Pr[SoundnessG(AWrapE(P), SchnorrVerifier).run(inzp (valR s)) @ &m : res].
+have -> : Pr[SoundnessG(AWrap(P), SchnorrVerifier).run(inzmod (valR s)) @ &m : res]
+ = Pr[SoundnessG(AWrapE(P), SchnorrVerifier).run(inzmod (valR s)) @ &m : res].
 byequiv. proc.  sim. auto. auto.
-apply (extractabilityG (AWrapE(P)) _ _ _ &m (inzp (valR s))).
+apply (extractabilityG (AWrapE(P)) _ _ _ &m (inzmod (valR s))).
 proc. call P_response_ll. auto.
 proc. call P_commitment_ll. auto.
 apply P_rewindable.
